src/pf2ir/PFRace.v
@@ -1,0 +1,41 @@
+From sflib Require Import sflib.
+From Paco Require Import paco.
+
+From PromisingLib Require Import Axioms.
+From PromisingLib Require Import Basic.
+From PromisingLib Require Import DataStructure.
+From PromisingLib Require Import DenseOrder.
+From PromisingLib Require Import Language.
+From PromisingLib Require Import Event.
+
+Require Import Time.
+Require Import View.
+Require Import BoolMap.
+Require Import Promises.
+Require Import Reserves.
+Require Import Cell.
+Require Import Memory.
+Require Import TView.
+Require Import Global.
+Require Import Local.
+Require Import Thread.
+Require Import Configuration.
+Require Import PFConfiguration.
+Require Import Behavior.
+
+Set Implicit Arguments.
+
+
+Variant pf_race (c0: Configuration.t): Prop :=
+| pf_race_intro
+    e tid c1 c2
+    (STEPS: PFConfiguration.all_step c0 c1)
+    (STEP: PFConfiguration.estep e tid c1 c2)
+    (RACE: ThreadEvent.is_race e)
+.
+
+Definition pf_racefree (c: Configuration.t): Prop :=
+  ~ pf_race c.
+
+Definition pf_racefree_syn (syn: Threads.syntax): Prop :=
+  pf_racefree (Configuration.init syn).
