src/prop/PFCertify.v
@@ -1,0 +1,51 @@
+From sflib Require Import sflib.
+From Paco Require Import paco.
+
+From PromisingLib Require Import Axioms.
+From PromisingLib Require Import Basic.
+From PromisingLib Require Import Loc.
+From PromisingLib Require Import DataStructure.
+From PromisingLib Require Import DenseOrder.
+From PromisingLib Require Import Language.
+From PromisingLib Require Import Event.
+
+Require Import Time.
+Require Import View.
+Require Import BoolMap.
+Require Import Promises.
+Require Import Reserves.
+Require Import Cell.
+Require Import Memory.
+Require Import TView.
+Require Import Global.
+Require Import Local.
+Require Import Thread.
+
+
+Section PFCertify.
+  Variable lang: language.
+
+  Variant pf_certify (loc: Loc.t) (th: Thread.t lang): Prop :=
+    | pf_certify_failure
+        pf e th1 th2
+        (STEPS: rtc (Thread.pf_tau_step (Global.max_reserved (Thread.global th))) th th1)
+        (STEP_FAILURE: Thread.step (Global.max_reserved (Thread.global th)) pf e th1 th2)
+        (EVENT_FAILURE: ThreadEvent.get_machine_event e = MachineEvent.failure)
+    | pf_certify_fulfill
+        pf e th1 th2
+        from to val released ord
+        (STEPS: rtc (Thread.pf_tau_step (Global.max_reserved (Thread.global th))) th th1)
+        (STEP_FULFILL: Thread.step (Global.max_reserved (Thread.global th)) pf e th1 th2)
+        (EVENT_FULFILL: ThreadEvent.is_writing e = Some (loc, from, to, val, released, ord))
+        (TO: Time.lt (Memory.max_ts loc (Global.memory (Thread.global th1))) to)
+        (ORD: Ordering.le ord Ordering.na)
+  .
+
+  Lemma consistent_pf_certify
+        th loc
+        (CONS: Thread.consistent th)
+        (PROMISED: th.(Thread.local).(Local.promises) loc = true):
+    pf_certify loc th.
+  Proof.
+  Admitted.
+End PFCertify.
